lib/fst/Lib.RawIntTypes.fst
@@ -39,3 +39,4 @@ let uint_to_nat #t (x:uint_t t) =
   | U64 -> UInt64.v x
   | U128 -> UInt128.v x
   | SIZE -> UInt32.v x
+  | NATm m -> x
